src/lectures/L07Axiomatic.md
@@ -986,4 +986,3 @@ but, lets be honest, the construction is a real PITA.
 
 Next, lets see how to dramatically automate these proofs using **verification conditions**.
 
-
