src/lectures/L08VerificationConditions.md
@@ -64,6 +64,22 @@ def erase (c : ACom) : Com :=
 
 As before we can define some "notation" to make it easier to write `ACom` programs.
 
+  |- {λ s => inv s /\ bval b s} c {λs => inv s}
+
+One lean-y way to say that `inv` is an invariant:
+
+∀ {s, t},
+  ⟨ c , s ⟩ ==> t ->
+  inv s ->
+  bval b s ->
+  inv t
+
+wp : Com -> Assertion -> Assertion
+
+{λ s => inv s /\ bval b s} ⊆ wp c inv
+
+
+
 ```lean
 notation:10 x "<~" e  => ACom.Assign x (ToAexp.toAexp e)
 infixr:20 ";;"  => ACom.Seq
@@ -71,7 +87,10 @@ notation:10 "IF" b "THEN" c1 "ELSE" c2 => ACom.If b c1 c2
 notation:12 "WHILE {-@" inv "@-}" b "DO" c "END" => ACom.While inv (ToBexp.toBexp b) c
 notation:20 "[|" c "|]" => erase c
 notation:10 "⊢" " {|" p "|}" c "{|" q "|}" => FH p (erase c) q
+
+-- REPEAT c UNTIL b == c ;; WHILE (not c) DO c END
 ```
+
 
 
 Specifically, note the `⊢ {| p |} c {| q |}` triple
@@ -104,7 +123,9 @@ def vc (c : ACom) (q : Assertion) : Prop :=
   | ACom.Assign _ _  => True
   | ACom.Seq c1 c2   => vc c1 (wp c2 q) /\ (vc c2 q)
   | ACom.If _ c1 c2  => vc c1 q /\ vc c2 q
-  | ACom.While i b c => (∀ s, i s -> bval b s -> wp c i s) /\
+  | ACom.While i b c =>
+                        -- ((λ s => i s /\ bval b s) ⊆ (wp c i)) /\
+                        (∀ s, i s -> bval b s -> wp c i s) /\
                         (∀ s, i s -> ¬ bval b s -> q s) /\
                         vc c i
 
@@ -114,7 +135,16 @@ theorem vc_sound : vc c q -> (⊢ {| wp c q |} c {| q |})
   induction c generalizing q
   . case Skip   => constructor
   . case Assign => constructor
-  . case Seq    => sorry
+  . case Seq    =>
+    rename_i c1 c2 ih1 ih2
+    simp [vc] at vcq
+    cases vcq
+    simp []
+    constructor
+    apply ih1
+    assumption
+    apply ih2
+    assumption
   . case If     => sorry
   . case While  => sorry
 
@@ -123,7 +153,7 @@ theorem vc_sound : vc c q -> (⊢ {| wp c q |} c {| q |})
 @[simp]
 def vc' (p: Assertion) (c: ACom) (q: Assertion) : Prop := (p ⊆ wp c q) ∧ (vc c q)
 
-theorem vc'_sound : vc' p c q -> (⊢ {{ p }} (erase c) {{ q }}) := by
+theorem vc'_sound : (vc' p c q) -> (⊢ {| p |} c {| q |}) := by
   intros vcq
   cases vcq
   rename_i vc1 vc2
@@ -134,86 +164,160 @@ theorem vc'_sound : vc' p c q -> (⊢ {{ p }} (erase c) {{ q }}) := by
 
 /- ----------------------------------------------------------------------------------------------- -/
 
-theorem ex_swap :
+theorem ex_swap : ∀ {a b},
   ⊢ {| λs => s x = a /\ s y = b |}
       (z <~ x) ;;
       (x <~ y) ;;
       (y <~ z)
     {| λs => s x = b /\ s y = a |}
   := by
-  apply vc'_sound; simp_all [aval, upd]
+  intros a b
+  apply vc'_sound
+  simp [vc', aval, upd]
+  intros; constructor <;> assumption
 
 /- ----------------------------------------------------------------------------------------------- -/
 
-theorem ex1 : ⊢ {| tt |}
-                  x <~ 5
-                {| λs => s x = 5 |}
-  := by
-  apply vc'_sound; simp_all [aval, upd]
-
-/- ----------------------------------------------------------------------------------------------- -/
-
-theorem ex2 : ⊢ {| λs => s x = 10 |}
-                  (x <~ x + 1) ;;
-                  (x <~ x + 1)
-                {| λs => s x = 12 |}
-  := by
-  apply vc'_sound; simp_all [aval, upd]
-
-/- ----------------------------------------------------------------------------------------------- -/
-
-
-theorem ex4 : ⊢ {| tt |}
-                WHILE {-@ tt @-} true DO
-                  Skip
-                END
-                {| ff |}
+theorem ex1 :
+  ⊢ {| tt |}
+    x <~ 5
+    {| λs => s x = 5 |}
   := by
   apply vc'_sound
-  simp_all [aval, bval]
+  simp_all [aval, upd]
 
 /- ----------------------------------------------------------------------------------------------- -/
+
+theorem ex2 :
+  ⊢ {| λs => s x = 10 /\ s y = 1 |}  -- (2) ??
+      (x <~ x + y) ;;
+      (x <~ x + y)
+    {| λs => s x = 12 |}  -- (1) ??
+  := by
+  apply vc'_sound; simp_all [aval, upd]
+
+-- (1) change POST to λ s => s x = 12 /\ s y = 1
+-- (2) change PRE  to λ s => s x = 10 /\ s y = 1
+
+/- ----------------------------------------------------------------------------------------------- -/
+
+
+theorem ex4 :
+  ⊢ {| tt |}
+    WHILE {-@ tt @-} true DO
+      Skip
+    END
+    {| ff |}
+  := by
+  apply vc'_sound
+  simp [vc', bval]
+
+/-
+vc' tt (while {tt} true skip) ff
+==
+vc (while {tt} true skip) ff
+
+-- (1) tt /\ true => (wp Skip inv)
+-- (2) tt /\ not true => ff
+
+-/
+  -- simp_all [aval, bval]
+
+/- ----------------------------------------------------------------------------------------------- -/
+
+-- x=100, 100+0, 100+0+1, 100+0+1+2, 100+0+1+2+3,... 100+0+1+2+3+...+(z-1)
 
 theorem ex_loop :
   ⊢ {| tt |}
-      (y <~ 0)
-      ;;
-      (x <~ 100)
-      ;;
-      (WHILE {-@ λ s => 100 <= s x /\ 0 <= s y @-} y << z DO
+      (y <~ 0)   ;;
+      (x <~ 100) ;;
+      (WHILE {-@ λs => 100 <= s x  @-} y << z DO
          ((x <~ x + y) ;;
-          (y <~ y - 1))
+          (y <~ y + 1))
       END)
     {| λ s => 100 <= s x |}
   := by
   apply vc'_sound
-  simp_all [aval, bval, upd]
-  intros s hx _
-  calc 100 <= s x       := by assumption
-       _   <= s x + s y := by simp_arith []
+  simp [bval, aval, upd]
+  constructor
+  . intros s x_100 _
+    calc 100 <= s x       := by assumption
+         _   <= s x + s y := by simp []
+  . intros; assumption
 
-theorem imp_sum' :
-  ⊢ {| λ s => s "x" = i |}
+
+/-
+(x:=n, y:=0)
+(x:=n-1, y := 1)
+(x:=n-2, y := 2)
+(x:=n-3, y := 3)
+...
+(x:=1,   y := n-1)
+(x:=0,   y := n)
+
+
+(x:=0,   y := n)
+-/
+
+theorem bob : ∀ {a b}, 0 < a -> a - 1 + (b + 1) = a + b := by
+  intros a b a_pos
+
+  cases a
+  . contradiction
+  . simp_arith []
+
+theorem ex_drain: ∀ {n: Nat},
+  ⊢ {| λ s => s x = n |}
+      (y <~ 0)
+      ;;
+      (WHILE {-@ λ s => s x + s y = n @-} 0 << x DO
+         ((x <~ x - 1) ;;
+          (y <~ y + 1))
+      END)
+    {| λ s => s y = n |}
+  := by
+  intro n
+  apply vc'_sound
+  simp [bval, aval, upd]
+  constructor
+  . intros s xy_n x_pos; simp [<-xy_n]; apply bob; assumption
+  . intros s xy_n x_0; simp_all[]
+
+/-
+x:=n, y:=0
+x:=n-1, y:=0 +)
+x:=n-2, y:=0 +n + (n-1)
+x:=n-3, y:=0 +n + (n-1) +(n-2)
+...
+x:=0  , y:=0 +n + (n-1) +(n-2)+ ...+ 1
+
+
+-/
+
+
+theorem imp_sum' : ∀ {n},
+  ⊢ {| λ s => s "x" = n |}
       (y <~ 0) ;;
-      (WHILE {-@ wsum_inv i @-} (0 << x) DO
+      (WHILE {-@ λs => s y + sum (s x) = sum n @-} (0 << x) DO
         (y <~ y + x) ;;
         (x <~ x - 1)
        END)
-    {| λ s => s "y" = sum i |}
+    {| λ s => s "y" = sum n |}
   := by
+  intros n
   apply vc'_sound
-  simp_all [aval, bval, wsum_inv, upd]
+  simp_all [aval, bval, upd]
   constructor <;> repeat constructor
   . case a.left =>
     intros
-    rename_i s _ _
+    rename_i s a b
     generalize hx : s x = vx
-    cases vx <;> simp_all [sum, Nat.add_assoc]
+    cases vx <;> simp_all [sum, Nat.add_assoc, Nat.add_comm]
+
   . case a.right =>
     intros
     rename_i s _ _
     generalize hx : s x = vx
     cases vx <;> simp_all [sum, Nat.add_assoc]
 ```
-
 
